<?xml version="1.0" encoding="UTF-8"?>
<rdf:RDF xmlns:rdf="http://www.w3.org/1999/02/22-rdf-syntax-ns#" xmlns:skos="http://www.w3.org/2004/02/skos/core#" xmlns:dc="http://purl.org/dc/elements/1.1/"><skos:ConceptScheme rdf:about="https://w3id.org/formater/variable/"><dc:title>MON THESAURUS MACHIN</dc:title><dc:description>Solid Earth Products</dc:description></skos:ConceptScheme><skos:Concept rdf:about="geomagnetism" xml:base="https://w3id.org/formater/variable/"><skos:prefLabel xml:lang="en">Geomagnetism</skos:prefLabel><skos:prefLabel xml:lang="fr">Géomagnétisme</skos:prefLabel><skos:definition xml:lang="en">The magnetism of the earth. Also known as terrestrial magnetism. 
</skos:definition><skos:definition xml:lang="fr">Le magnétisme terrestre</skos:definition><skos:broader rdf:resource="solid_earth"/><skos:narrower rdf:resource="geomagnetism-geomagnetic_indices"/><skos:narrower rdf:resource="geomagnetism-geomagnetic_events"/><skos:narrower rdf:resource="geomagnetism-reference_fields"/><skos:narrower rdf:resource="geomagnetism-magnetic_field"/><skos:narrower rdf:resource="geomagnetism-paleomagnetism"/><skos:narrower rdf:resource="geomagnetism-electrical_field"/><skos:narrower rdf:resource="geomagnetism-geomagnetic_forecasts"/><skos:exactMatch rdf:resource="https://gcmdservices.gsfc.nasa.gov/kms/concept/910013d7-1e6a-4d1a-9921-be32d792a290"/></skos:Concept><skos:Concept rdf:about="geomagnetism-geomagnetic_indices" xml:base="https://w3id.org/formater/variable/"><skos:prefLabel xml:lang="en">Geomagnetic indices</skos:prefLabel><skos:prefLabel xml:lang="fr">Indices d'activité magnétique</skos:prefLabel><skos:definition xml:lang="en">Magnetic activity indicies that describe variations in the geomagnetic field, caused by irregular current systems occurring in the magnetosphere, ionosphere and deep in the Earth, in their own unique way.Typical magnetic activity indices are, from polar regions up to equatorial ones: PC, AE, aa, am, Kp and Dst.</skos:definition><skos:definition xml:lang="fr">Indices d'activité magnétique qui décrivent les variations du champ géomagnétique causées par des systèmes de courant irréguliers se produisant dans la magnétosphère, l'ionosphère et les profondeurs de la Terre, de façon unique.
Les indices d'activité magnétique typiques sont, des régions polaires aux régions équatoriales : PC, AE, aa, aa, am, Kp et Dst.</skos:definition><skos:broader rdf:resource="geomagnetism"/><skos:narrower rdf:resource="geomagnetism-geomagnetic_indices-aa_index"/><skos:narrower rdf:resource="geomagnetism-geomagnetic_indices-am_index"/><skos:narrower rdf:resource="geomagnetism-geomagnetic_indices-kp_index"/><skos:narrower rdf:resource="geomagnetism-geomagnetic_indices-dst_index"/><skos:narrower rdf:resource="geomagnetism-geomagnetic_indices-ae_index"/><skos:narrower rdf:resource="geomagnetism-geomagnetic_indices-pc_index"/><skos:exactMatch rdf:resource="https://gcmdservices.gsfc.nasa.gov/kms/concept/ae35f430-6534-49de-8b4c-edfc1e98870a"/></skos:Concept><skos:Concept rdf:about="geomagnetism-geomagnetic_indices-aa_index" xml:base="https://w3id.org/formater/variable/"><skos:prefLabel xml:lang="en">aa index</skos:prefLabel><skos:prefLabel xml:lang="fr">indice aa</skos:prefLabel><skos:definition xml:lang="en">aa (type of index: K-derived planetary; time resolution: 3-hour UT interval; unit: nT; availability: from 1868 onwards)  is derived from the K indices calculated at two nearly antipodal observatories to measure the amplitude of global geomagnetic activity during 3-hour intervals normalized to geomagnetic latitude ±50°. aa was introduced to monitor geomagnetic activity over the longest possible time period. aa and related deived geomagnetic indices such as: Aa, Kpa, CK24 and CK48) are provided by the Ecole et Observatoire des Sciences de la Terre, Strasbourg, France. aa time series is formally recognised and endorsed since 1975 by International Association of Geomagnetism and Aeronomy (IAGA).

                        </skos:definition><skos:definition xml:lang="fr">aa (type d'indice : Planétaire dérivé de K ; résolution temporelle : intervalle de 3 heures UT ; unité : nT ; disponibillité : depuis 1868) est dérivé des indices K calculés à deux observatoires quasi antipodaux pour mesurer l'amplitude de l'activité géomagnétique globale, pendant des intervalles tri-horaires, normalisée à la latitude géomagnétique ±50°. aa a été introduit pour surveiller l'activité géomagnétique sur la plus longue période possible. aa et les indices dérivés connexes (tels: Aa, Kpa, CK24 et CK48) sont fournis par l'Ecole et Observatoire des sciences de la Terre, Strasbourg, France. La série des indices aa est officiellement reconnue et labellisée depuis 1975 par l'Association internationale de géomagnétisme et d'aéronomie (IAGA).
</skos:definition><skos:broader rdf:resource="geomagnetism-geomagnetic_indices"/><skos:exactMatch rdf:resource="https://gcmdservices.gsfc.nasa.gov/kms/concept/5fd5ccc2-5edb-4823-940d-03a290a5c5fc"/></skos:Concept><skos:Concept rdf:about="geomagnetism-geomagnetic_indices-am_index" xml:base="https://w3id.org/formater/variable/"><skos:prefLabel xml:lang="en">am index</skos:prefLabel><skos:prefLabel xml:lang="fr">indice am</skos:prefLabel><skos:definition xml:lang="en">am (type of index: K-derived planetary and hemispheric; time resolution: 3-hour (UT) interval; unit: nT; availability: from 1959 onwards) is derived from the K indices calculated at a network of 24 magnetic observatories situated close to 50° corrected geomagnetic latitude (in the subauroral zones) covering all longitudes. am was introduced to allow a characterization of global geomagnetic activity using a large set of stations representing all longitudes and possible hemispheric discrepancies. am and related derived geomagnetic indices (such as: an, as, Kpm, Am, An and As) are provided by the Ecole et Observatoire des Sciences de la Terre, Strasbourg, France. am time series is formally recognised and endorsed since 1969 by International Association of Geomagnetism and Aeronomy (IAGA).
</skos:definition><skos:definition xml:lang="fr">am (type d'indice : Planétaire et hémisphérique dérivé des indices K ; résolution temporelle : Intervalle de 3 heures UT ; unité : nT ; disponibilité : à partir de 1959) est calculé à partir des indices K calculés sur un réseau de 24 observatoires magnétiques situés à une latitude géomagnétique corrigée proche de 50° (dans les zones subaurorales) et couvrant toutes les longitudes. am a été introduit pour permettre une caractérisation de l'activité géomagnétique globale utilisant un large ensemble de stations représentant toutes les longitudes et les possibles écarts hémisphériques. am et les indices dérivés connexes (tels: an, as, Kpm, Am, An et As) sont fournis par l'École et Observatoire des Sciences de la Terre, Strasbourg, France. La série des indices am est officiellement reconnue et labellisée depuis 1969 par l'Association internationale de géomagnétisme et d'aéronomie (IAGA).</skos:definition><skos:broader rdf:resource="geomagnetism-geomagnetic_indices"/><skos:exactMatch rdf:resource="https://gcmdservices.gsfc.nasa.gov/kms/concept/b3283844-d867-4c2f-9917-a72bc06fd9ef"/></skos:Concept><skos:Concept rdf:about="geomagnetism-geomagnetic_indices-kp_index" xml:base="https://w3id.org/formater/variable/"><skos:prefLabel xml:lang="en">Kp index</skos:prefLabel><skos:prefLabel xml:lang="fr">indice Kp</skos:prefLabel><skos:definition xml:lang="en">Kp (type of index: K-derived planetary; time resolution: 3-hour UT interval; unit: quasi-logarithmic scale as a third of K units, 28 values as
0o, 0+, 1-, 1o, 1+, 2-, up to 9o; availability: from 1932 onwards) is derived from the K indices calculated at a network of 11 northern and 2 southern stations between 44° and 60° northern or southern geomagnetic latitude. Kp was introduced to characterize the intensity of geomagnetic activity on a planetary scale, however because of the historical context at the time of its creation, the Kp network is heavily weighted towards Europe and Northern America. 
Kp and related derived indices (such as: ap, Ap, Cp and C9) are provided by the Helmholtz-Zentrum Potsdam, Deutsches GeoForschungsZentrum, Adolf-Schmidt-Observatorium, Niemegk, Germany. Kp time series is formally recognised and endorsed since 1954 by International Association of Geomagnetism and Aeronomy (IAGA).</skos:definition><skos:definition xml:lang="fr">Kp (type d'indice : Planétaire dérivé de K ; résolution temporelle : Intervalle de 3 heures UT) ; unité : échelle quasi-logarithmique de tiers d'unité K soit 28 valeurs : 0o, 0+, 1-, 1o, 1o, 1+, 2-, jusqu'à 9o. ; disponibilité : à partir de 1932) est calculé à partir des indices K d'un réseau de 11 stations nord et 2 stations sud entre 44° et 60° de latitudes géomagnétiques nord ou sud. Kp a été introduit pour caractériser l'intensité de l'activité géomagnétique à l'échelle planétaire, mais en raison du contexte historique au moment de sa création, le réseau Kp est fortement biaisé vers l'Europe et l'Amérique du Nord. 
Kp et les indices dérivés connexes (tels : ap, Ap, Cp et C9) sont fournis par le Helmholtz-Zentrum Potsdam, Deutsches GeoForschungsZentrum, Adolf-Schmidt-Observatorium, Niemegk, Allemagne.  La série des indices Kp est officiellement reconnue et labellisée depuis 1954 par l'Association internationale de géomagnétisme et d'aéronomie (IAGA).</skos:definition><skos:broader rdf:resource="geomagnetism-geomagnetic_indices"/><skos:exactMatch rdf:resource="https://gcmdservices.gsfc.nasa.gov/kms/concept/40386eea-beb0-4b83-906b-75c6bfa24b73"/></skos:Concept><skos:Concept rdf:about="geomagnetism-geomagnetic_indices-dst_index" xml:base="https://w3id.org/formater/variable/"><skos:prefLabel xml:lang="en">Dst index</skos:prefLabel><skos:prefLabel xml:lang="fr">indice Dst</skos:prefLabel><skos:definition xml:lang="en">Name "Dst" came from "Disturbance storm-time". Dst (type of index: Equatorial index horizontal component disturbances; time resolution: 1-hour UT interval; unit: nT; availability: from 1957 onwards)  is computed using 1-hour values from four low latitude observatories. Dst aims at monitoring the axis-symmetric magnetic signature of magnetosphere currents, including mainly the ring current, the tail currents and also the magnetopause Chapman-Ferraro current. At a given time, the Dst index is the average of variation over all longitudes; the reference level is set so that Dst is statistically zero on quiet days. An index of -50 or deeper indicates a storm-level disturbance, and an index of -200 or deeper is associated with middle-latitude auroras. Dst is determined by the World Data Center for Geomagnetism, Data Analysis Center for Geomagnetism and Space Magnetism, Kyoto University, Kyoto Japan. Dst time series is formally recognised and endorsed since 1969 by International Association of Geomagnetism and Aeronomy (IAGA).</skos:definition><skos:definition xml:lang="fr">Le nom "Dst" provient de l'acronyme anglophone "Disturbance storm-time". Dst (type d'index : Perturbations de la composante horizontale de l'indice équatorial ; résolution temporelle : Intervalle UT d'une heure ; unité : nT ; disponibilité : à partir de 1957) est calculé en utilisant les valeurs horaires de quatre observatoires de basse latitude. Dst vise à surveiller la signature magnétique axisymétrique des courants magnétosphériques, y compris principalement le courant annulaire, les courants de queue et aussi le courant de Chapman-Ferraro de la magnétopause. A un temps donné, l'indice Dst est la moyenne des variations sur toutes les longitudes ; le niveau de référence est fixé de sorte que Dst est statistiquement nul les jours calmes.  Un indice de -50 ou plus indique une perturbation de type orage magnétique, et un indice de -200 ou plus est associé à un orage intense présentant des aurores possibles même aux moyennes latitudes. Dst est déterminé par le World Data Center for Geomagnetism, Data Analysis Center for Geomagnetism and Space Magnetism, Kyoto University, Kyoto Japan.  La série des indices Dst est officiellement reconnue et labellisée depuis 1969 par l'Association internationale de géomagnétisme et d'aéronomie (IAGA).</skos:definition><skos:broader rdf:resource="geomagnetism-geomagnetic_indices"/><skos:exactMatch rdf:resource="https://gcmdservices.gsfc.nasa.gov/kms/concept/cdb4b514-75c4-4a1f-a4ad-1855fbd396ab"/><skos:exactMatch rdf:resource="http://doi.org/10.17593/14515-74000"/></skos:Concept><skos:Concept rdf:about="geomagnetism-geomagnetic_indices-ae_index" xml:base="https://w3id.org/formater/variable/"><skos:prefLabel xml:lang="en">AE index</skos:prefLabel><skos:prefLabel xml:lang="fr">indice AE</skos:prefLabel><skos:definition xml:lang="en">AE (type of index: Auroral index horizontal component disturbances; time resolution: 1-hour UTinterval from 1957 to 1965 ; 1-minute UT interval over periods 1966 to 1975, 1978 to June 1988, March 1989 and from 1990 onwards; unit: nT)  is computed using 1-minute values from 12 observatories in the Northern auroral zone. AE aims at monitor the magnetic signature of the eastward and westward auroral electrojets in the Northern hemisphere. The magnetograms of the horizontal components from the AE stations are 'superimposed', the upper envelope defines the AU index, and the lower envelope define the AL index; then AE = (AU - AL) and A0 = (AU + AL)/2.
AE and related derived geomagnetic indices (such as: AU, AL, A0) are determined by the World Data Center for Geomagnetism, Data Analysis Center for Geomagnetism and Space Magnetism, Kyoto University, Kyoto Japan.  AE time series is formally recognised and endorsed since 1969 by International Association of Geomagnetism and Aeronomy (IAGA).


</skos:definition><skos:definition xml:lang="fr">AE (type d'indice : Perturbations de la composante horizontale de l'indice auroral ; résolution temporelle : Intervalle UT d'une heure de 1957 à 1965 ; intervalle UT d'une minute sur les périodes 1966 à 1975, 1978 à juin 1988, mars 1989 et à partir de 1990 ; unité : nT) est calculé à partir des valeurs minute de 12 observatoires de la zone aurorale nord. AE vise à surveiller la signature magnétique des électrojets auroraux de l'hémisphère Nord vers l'est et vers l'ouest. Les magnétogrammes des composantes horizontales des stations AE sont " superposés ", l'enveloppe supérieure définit l'indice AU et l'enveloppe inférieure définit l'indice AL, puis AE = (AU - AL) et A0 = (AU + AL)/2.
AE et les indices géomagnétiques dérivés (tels : AU, AL, A0) sont déterminés par le World Data Center for Geomagnetism, Data Analysis Center for Geomagnetism and Space Magnetism, Kyoto University, Kyoto Japan. La série des indices AE est officiellement reconnue et labellisée depuis 1969 par l'Association internationale de géomagnétisme et d'aéronomie (IAGA).</skos:definition><skos:broader rdf:resource="geomagnetism-geomagnetic_indices"/><skos:exactMatch rdf:resource="https://gcmdservices.gsfc.nasa.gov/kms/concept/31f77d6b-72f7-45e6-93be-8ac5fd5dc373"/><skos:exactMatch rdf:resource="http://doi.org/10.17593/15031-54800"/></skos:Concept><skos:Concept rdf:about="geomagnetism-geomagnetic_indices-pc_index" xml:base="https://w3id.org/formater/variable/"><skos:prefLabel xml:lang="en">PC index</skos:prefLabel><skos:prefLabel xml:lang="fr">indice PC</skos:prefLabel><skos:definition xml:lang="en">PC (type of index: Polar Cap index horizontal component disturbances; time resolution: 1-minute UT interval, North PCN from 1975 and South PCS from 1995 onwards; unit: mV/m) is deduced from the deviations in the horizontal H and D magnetic field components from the quiet level at two polar cap stations (Thule and Vostok for respectively the PCN and PCS).
PC aims at monitor the geomagnetic activity over the polar caps caused by changes in the interplanetary magnetic field (IMF) and solar wind, driven by the geoeffective interplanetary electric field irrespective of time, season and solar cycle.
PCN is determined by the National Space Institute, Technical University of Denmark (DTU), Denmark; PCS is determined by the Arctic and Antarctic Research Institute (AARI), Russian Federation. PC time series is formally recognised and endorsed since 2013 by International Association of Geomagnetism and Aeronomy (IAGA).</skos:definition><skos:definition xml:lang="fr">PC (type d'index : indice des calottes polaires mesurant les perturbations de la composante horizontale du champ magnétique; résolution temporelle : Intervalle UT d'une minute, PCN Nord à partir de 1975 et PCS Sud à partir de 1995 ; unité : mV/m) est déduit des déviations des composantes horizontales H et D du champ magnétique par rapport au niveau en période calme dans deux stations polaires (Thule et Vostok pour respectivement les PCN et PCS). PC vise à permettre la surveillance de l'activité géomagnétique sur les calottes polaires provoquée par les changements du champ magnétique interplanétaire et du vent solaire, actionnés par le champ électrique interplanétaire géoefficace indépendamment du temps, de la saison et du cycle solaire.
Le PCN est calculé par le National Space Institute, Technical University of Denmark (DTU), Danemark; le PCS est calculé par l'Arctic and Antarctic Research Institute (AARI), Fédération de Russie. La série des indices PC est officiellement reconnue et labellisée depuis 2013 par l'Association internationale de géomagnétisme et d'aéronomie (IAGA).</skos:definition><skos:broader rdf:resource="geomagnetism-geomagnetic_indices"/></skos:Concept><skos:Concept rdf:about="geomagnetism-geomagnetic_events" xml:base="https://w3id.org/formater/variable/"><skos:prefLabel xml:lang="en">Magnetic remarkable events
</skos:prefLabel><skos:prefLabel xml:lang="fr">évênement magnétique remarquable</skos:prefLabel><skos:definition xml:lang="en">Magnetic remarkable events that have been measured at the Earth's surface in magnetic observatories and listed by geomagnetic community</skos:definition><skos:definition xml:lang="fr">Événements magnétiques remarquables mesurés à la surface de la Terre dans des observatoires magnétiques et répertoriés par la communauté en géomagnétisme</skos:definition><skos:broader rdf:resource="geomagnetism"/><skos:narrower rdf:resource="geomagnetism-geomagnetic_events-sc"/><skos:narrower rdf:resource="geomagnetism-geomagnetic_events-sfe"/><skos:narrower rdf:resource="geomagnetism-geomagnetic_events-qday"/><skos:narrower rdf:resource="geomagnetism-geomagnetic_events-dday"/><skos:exactMatch rdf:resource="https://gcmdservices.gsfc.nasa.gov/kms/concept/ae35f430-6534-49de-8b4c-edfc1e98870a"/></skos:Concept><skos:Concept rdf:about="geomagnetism-geomagnetic_events-sc" xml:base="https://w3id.org/formater/variable/"><skos:prefLabel xml:lang="en">Sudden Commencement (SC)</skos:prefLabel><skos:prefLabel xml:lang="fr">Soudain Commencement (SC)</skos:prefLabel><skos:definition xml:lang="en">Sudden commencement followed by a magnetic storm/an increase in activity (SSC - Storm Sudden Commencement) or by no further disturbance (SI - Sudden Impulse). A SC is basically an unexpected sharp increase in the Northern (X) magnetic component of a considered observatory. Usually, but not always a SC is the precursor to a geomagnetic storm (defined by, for example, a minimum of the Dst index). It has to be noted that more emphasis is put on the change of rhythm in the magnetic activity than on the amplitude of the possible succeeding magnetic storm. The SC list is available from 1868 onwards and made available by Observatori de l'Ebre (Spain). The SC list is formally recognised and endorsed since 1975 by International Association of Geomagnetism and Aeronomy (IAGA).</skos:definition><skos:definition xml:lang="fr">Début soudain suivi d'un orage magnétique/d'une augmentation de l'activité (SSC - Storm Sudden Commencement) ou d'aucune activité magnétique majeure (SI - Sudden Impulse). Un SC est fondamentalement une forte augmentation inattendue de la composante magnétique Nord (X) à la position d'un observatoire. Habituellement, mais pas toujours, un SC est le précurseur d'un orage magnétique (défini, par exemple, par un minimum de l'indice Dst). Il faut noter que l'accent est davantage mis sur le changement de rythme de l'activité magnétique que sur l'amplitude de l'éventuel orage magnétique. La liste des SCs est disponible à partir de 1868 et mise à disposition par Observatori de l'Ebre (Espagne). La liste des SCs est officiellement reconnue et labellisée depuis 1975 par l'Association Internationale de Géomagnétisme et d'Aéronomie (IAGA).</skos:definition><skos:broader rdf:resource="geomagnetism-geomagnetic_events"/></skos:Concept><skos:Concept rdf:about="geomagnetism-geomagnetic_events-sfe" xml:base="https://w3id.org/formater/variable/"><skos:prefLabel xml:lang="en">Solar Flare Event (SFE)</skos:prefLabel><skos:prefLabel xml:lang="fr">événement d'éruption solaire</skos:prefLabel><skos:definition xml:lang="en">Solar Flare Effects when solar flare points towards the Earth. SFE are usually noticed as the signature on magnetograms at low and mid-latitude stations of an increase in the intensity of the Solar-quiet current system. The events are characterised by visual analysis of conditions on the Sun. When a solar flare points towards the Earth,  SFE events occur. Preliminary lists of  SFE events are compiled on the basis of reports made by observatories by morphological inspection of their magnetograms. Definitive lists of  SFE events are based on reports from observatories in response to a checking list sent by Observatori de l'Ebre, Spain. The SFE list is available from 1970 onwards and made available by Observatori de l'Ebre (Spain). The SFE list is formally recognised and endorsed since 1975 by International Association of Geomagnetism and Aeronomy (IAGA).</skos:definition><skos:definition xml:lang="fr">Effets des éruptions solaires lorsque celles-ci impactent la Terre. Un SFE est généralement observé sur les magnétogrammes des stations de basses et moyennes latitudes comme une augmentation de l'intensité du système de courants des conditions calmes (solar-quiet). Les événements sont caractérisés par l'analyse visuelle des conditions sur le Soleil. Lorsqu'une éruption solaire pointe vers la Terre, des événements SFE se produisent. Des listes préliminaires d'événements sont établies sur la base des rapports établis par les observatoires suite aux inspections morphologiques de leurs magnétogrammes. Les listes définitives des événements SFE sont basées sur les rapports des observatoires contrôlés et synthétisés par Observatori de l'Ebre, Espagne. La liste des SFE est disponible à partir de 1970 et mise à disposition par Observatori de l'Ebre (Espagne). La liste SFE est officiellement reconnue et approuvée depuis 1975 par l'Association internationale de géomagnétisme et d'aéronomie (IAGA).
</skos:definition><skos:broader rdf:resource="geomagnetism-geomagnetic_events"/></skos:Concept><skos:Concept rdf:about="geomagnetism-geomagnetic_events-qday" xml:base="https://w3id.org/formater/variable/"><skos:prefLabel xml:lang="en">Quiet day</skos:prefLabel><skos:prefLabel xml:lang="fr">Jour calme</skos:prefLabel><skos:definition xml:lang="en">A day of magnetic quietness, when the daily magnetograms of observatories on the Earth's surface show only diurnal variations due to the day/night alternance.</skos:definition><skos:definition xml:lang="fr">Jour de calme magnétique, lorsque les magnétogrammes journalier des observatoires à la surface de la Terre ne montrent que des variations diurnes dues à l'alternance jour/nuit. </skos:definition><skos:broader rdf:resource="geomagnetism-geomagnetic_events"/></skos:Concept><skos:Concept rdf:about="geomagnetism-geomagnetic_events-dday" xml:base="https://w3id.org/formater/variable/"><skos:prefLabel xml:lang="en">Disturbed day</skos:prefLabel><skos:prefLabel xml:lang="fr">Jour perturbé
</skos:prefLabel><skos:definition xml:lang="en">A day of magnetic disturbance, when the daily magnetograms of observatories on the Earth's surface show irregular geomagnetic activity </skos:definition><skos:definition xml:lang="fr">Jour perturbé magnétiquement, lorsque les magnétogrammes journaliers des observatoires à la surface de la Terre montrent une activité géomagnétique irrégulière. </skos:definition><skos:broader rdf:resource="geomagnetism-geomagnetic_events"/></skos:Concept><skos:Concept rdf:about="geomagnetism-reference_fields" xml:base="https://w3id.org/formater/variable/"><skos:prefLabel xml:lang="en">Reference field</skos:prefLabel><skos:prefLabel xml:lang="fr">Champ de référence</skos:prefLabel><skos:definition xml:lang="en">Reference models of the Earth's magnetic field (core, crustal, ionospheric or magnetospheric field) that serves as a common recognised representation</skos:definition><skos:definition xml:lang="fr">Modèles de référence du champ magnétique terrestre (principal, crustal, ionosphérique ou magnétosphérique) servant de représentation commune reconnue.</skos:definition><skos:broader rdf:resource="geomagnetism"/><skos:narrower rdf:resource="geomagnetism-reference_fields-igrf"/><skos:narrower rdf:resource="geomagnetism-reference_fields-wdmam"/><skos:exactMatch rdf:resource="https://gcmdservices.gsfc.nasa.gov/kms/concept/fd631e31-fe6f-462e-a3f6-c07b4b736ac7"/></skos:Concept><skos:Concept rdf:about="geomagnetism-reference_fields-igrf" xml:base="https://w3id.org/formater/variable/"><skos:prefLabel xml:lang="en">International Geomagnetic Reference Field Model (IGRF)</skos:prefLabel><skos:prefLabel xml:lang="fr">Modèle international géomagnétique de référence</skos:prefLabel><skos:definition xml:lang="en">Standard and international mathematical description of the Earth's main magnetic field.  
The Internal field (main field)  is modelled in spherical harmonics up to degree/order 13 from 1900.0 onwards with a time resolution of 5 years interval. An international task force, under the auspices of the International Association of Geomagnetism and Aeronomy Working Group (namely  IAGA division V Working Group "V-MOD: Geomagnetic Field Modeling"), produces a new generation of the IGRF. Thus, it is the product of a collaborative effort between magnetic field modellers and the institutes involved in acquiring, collecting and disseminating magnetic field data from satellites, observatories and surveys around the world. IGRF is used widely in studies of the Earth's deep interior, its crust, its ionosphere and magnetosphere as well as by industrial stakeholders for navigational applications, oil and mining exploration, etc</skos:definition><skos:definition xml:lang="fr">Description mathématique standard et internationale du champ magnétique principal de la Terre.  
Le champ interne (champ principal) est modélisé en harmoniques sphériques jusqu'au degré/ordre 13 à partir de 1900.0 avec une résolution temporelle de 5 ans. Un groupe de travail international, sous les auspices de l'Association Internationale de Géomagnétisme et d'Aéronomie (à savoir le groupe de travail "V-MOD : Geomagnetic Field Modeling" de l'IAGA division V), produit une nouvelle génération du IGRF. L'IGRF est donc le fruit d'un effort de collaboration entre les modélisateurs de champs magnétiques et les instituts impliqués dans l'acquisition, la collecte et la diffusion de données de champs magnétiques provenant de satellites, d'observatoires et d'enquêtes dans le monde entier. L'IGRF est largement utilisé dans les études de la Terre solide, de la croûte terrestre, de l'ionosphère et de la magnétosphère ainsi que par les acteurs du monde industriel pour les applications de navigation, d'exploration pétrolière et minière, etc. 
</skos:definition><skos:broader rdf:resource="geomagnetism-reference_fields"/></skos:Concept><skos:Concept rdf:about="geomagnetism-reference_fields-wdmam" xml:base="https://w3id.org/formater/variable/"><skos:prefLabel xml:lang="en">World Digital Magnetic anomaly Map (WDMAM)</skos:prefLabel><skos:prefLabel xml:lang="fr">Carte Mondiale digitale des anomalies magnétiques </skos:prefLabel><skos:definition xml:lang="en">The World Digital Magnetic Anomaly Map is an international scientific project under the auspices of International Association of Geomagnetism and Aeronomy (IAGA) and the Commission for the Geological Map of the World (CGMW), aiming to compile and make available magnetic anomalies caused by the Earth lithosphere, on continental and oceanic areas, in a comprehensive way, all over the World.

 The WDMAM is a grid given in a reference geodetic system which spatial resolution is adapted but coherent among  available datasets: small spatial scales where local surveys are available, long wavelengths derived from satellite data and models. The first version was delivered in 2003.</skos:definition><skos:definition xml:lang="fr">La Carte Mondiale digitale des anomalies magnétiques est un projet scientifique international sous les auspices de l'Association internationale de Géomagétisme et d'Aéronomie (IAGA) et de la Comission de la Carte Géologique du Monde (CGMW (Commission for the Geological Map of the World), visant à compiler et rendre disponibles les anomalies magnétiques dues à la lithosphère terrestre, dans les zones continentales et océaniques, de manière exhaustive, partout dans le monde.  Le WDMAM est une grille donnée dans un système géodésique de référence dont la résolution spatiale est adaptée mais cohérente entre les ensembles de données disponibles : petites échelles spatiales où des relevés locaux sont disponibles, grandes longueurs d'onde dérivées des données satellitaires et modèles. La première version fut rendue disponible en 2003.</skos:definition><skos:broader rdf:resource="geomagnetism-reference_fields"/></skos:Concept><skos:Concept rdf:about="geomagnetism-magnetic_field" xml:base="https://w3id.org/formater/variable/"><skos:prefLabel xml:lang="en">Magnetic field</skos:prefLabel><skos:prefLabel xml:lang="fr">Champ magnétique</skos:prefLabel><skos:definition xml:lang="en">Pertaining to the magnetic field generated by the Earth and its environment</skos:definition><skos:definition xml:lang="fr">Fait référence au champ magnétique généré par la Terre et son environnement proche </skos:definition><skos:broader rdf:resource="geomagnetism"/><skos:narrower rdf:resource="geomagnetism-magnetic_field-magnetic_declination"/><skos:narrower rdf:resource="geomagnetism-magnetic_field-magnetic_induction"/><skos:narrower rdf:resource="geomagnetism-magnetic_field-magnetic_anomalies"/><skos:narrower rdf:resource="geomagnetism-magnetic_field-magnetic_inclination"/><skos:narrower rdf:resource="geomagnetism-magnetic_field-magnetic_intensity"/><skos:narrower rdf:resource="geomagnetism-magnetic_field-magnetic_components"/><skos:exactMatch rdf:resource="https://gcmdservices.gsfc.nasa.gov/kms/concept/204b482b-449b-42c9-a5bb-f6da42bee3a4"/></skos:Concept><skos:Concept rdf:about="geomagnetism-magnetic_field-magnetic_declination" xml:base="https://w3id.org/formater/variable/"><skos:prefLabel xml:lang="en">Magnetic declination</skos:prefLabel><skos:prefLabel xml:lang="fr">Déclinaison magnétique</skos:prefLabel><skos:definition xml:lang="en">Angle of magnetic North direction from geographical North, expressed in degrees, positive towards East.

</skos:definition><skos:definition xml:lang="fr">Angle de la direction nord magnétique par rapport au nord géographique, exprimé en degrés, positif vers l'est.
</skos:definition><skos:broader rdf:resource="geomagnetism-magnetic_field"/><skos:exactMatch rdf:resource="https://gcmdservices.gsfc.nasa.gov/kms/concept/f311eac7-5c85-4a8f-90c2-abcff3eec92d"/></skos:Concept><skos:Concept rdf:about="geomagnetism-magnetic_field-magnetic_induction" xml:base="https://w3id.org/formater/variable/"><skos:prefLabel xml:lang="en">magnetic induction</skos:prefLabel><skos:prefLabel xml:lang="fr">induction magnétique</skos:prefLabel><skos:definition xml:lang="en">Geomagnetic electromotive force generated in a closed circuit by a change in the flow of currents.magnetic induction is the production of an electromotive force (i.e., voltage) across an electrical conductor in a changing magnetic field.
</skos:definition><skos:definition xml:lang="fr"/><skos:broader rdf:resource="geomagnetism-magnetic_field"/><skos:exactMatch rdf:resource="https://gcmdservices.gsfc.nasa.gov/kms/concept/ee421700-0fe2-420c-9a07-91e8ae9fb524"/></skos:Concept><skos:Concept rdf:about="geomagnetism-magnetic_field-magnetic_anomalies" xml:base="https://w3id.org/formater/variable/"><skos:prefLabel xml:lang="en">Magnetic anomalies</skos:prefLabel><skos:prefLabel xml:lang="fr">Anomalies magnétiques</skos:prefLabel><skos:definition xml:lang="en">Local variation of the Earth's magnetic field from the expected value at this location. The expected value can be that determined from main magnetic field models, and magnetic anomalies therefore result from local deposits of remanent magnetic materials in the rocks of the Earth's crust. The magnetic variation in successive bands of seafloor lineations, parallel to ridges, is the founding evidence of seafloor spreading theory, central to plate tectonics.</skos:definition><skos:definition xml:lang="fr">Variation locale du champ magnétique terrestre par rapport à la valeur attendue à cet endroit. La valeur attendue peut être celle déterminée à partir de modèles de champ magnétique principal, et, les anomalies magnétiques résultent donc de dépôts locaux de matériaux magnétiques rémanents dans les roches de la croûte terrestre. La variation magnétique en bandes succéssives des linéations des fonds océaniques, parallèles aux dorsales, est la preuve fondatrice de la théorie de l'expansion des fonds océaniques, au centre de la tectonique des plaques.
</skos:definition><skos:broader rdf:resource="geomagnetism-magnetic_field"/><skos:exactMatch rdf:resource="https://gcmdservices.gsfc.nasa.gov/kms/concept/65ae8ab2-489b-44bf-bf5b-43cf957b70c0"/></skos:Concept><skos:Concept rdf:about="geomagnetism-magnetic_field-magnetic_inclination" xml:base="https://w3id.org/formater/variable/"><skos:prefLabel xml:lang="en">Magnetic inclination</skos:prefLabel><skos:prefLabel xml:lang="fr">Inclinaison Magnétique</skos:prefLabel><skos:definition xml:lang="en">The dip angle that the vector magnetic field makes with the horizontal plane (determined with regards to geoide or reference ellipsoid), expressed in degrees, positive towards  Earth's center.</skos:definition><skos:definition xml:lang="fr">L'angle de pendage que le champ magnétique vectoriel fait avec le plan horizontal (déterminé par rapport au géoïde ou à l'ellipsoïde de référence), exprimé en degrés, positif vers le centre de la Terre.</skos:definition><skos:broader rdf:resource="geomagnetism-magnetic_field"/><skos:exactMatch rdf:resource="https://gcmdservices.gsfc.nasa.gov/kms/concept/f0b7311e-df08-45fa-8dd5-33b6f74a66d9"/></skos:Concept><skos:Concept rdf:about="geomagnetism-magnetic_field-magnetic_intensity" xml:base="https://w3id.org/formater/variable/"><skos:prefLabel xml:lang="en">Magnetic intensity</skos:prefLabel><skos:prefLabel xml:lang="fr">Intensité du champ magnétique</skos:prefLabel><skos:definition xml:lang="en">Strength of the Earth's magnetic field. In a point, is equivalent to the square root of the sum of the squares of the components of the magnetic vector field in this point.</skos:definition><skos:definition xml:lang="fr">Intensité, force du champ magnétique terrestre. En un point, est équivalent à la racine carrée de la somme des carrés des composantes du champ magnétique vectoriel en ce point.</skos:definition><skos:broader rdf:resource="geomagnetism-magnetic_field"/><skos:exactMatch rdf:resource="https://gcmdservices.gsfc.nasa.gov/kms/concept/d817911a-685b-4c9f-bdc7-2411b8c0a7af"/></skos:Concept><skos:Concept rdf:about="geomagnetism-magnetic_field-magnetic_components" xml:base="https://w3id.org/formater/variable/"><skos:prefLabel xml:lang="en">Magnetic components</skos:prefLabel><skos:prefLabel xml:lang="fr">Composantes du champ magnétique</skos:prefLabel><skos:definition xml:lang="en">The coordinates of the magnetic field vector at a point in space outside the conventionally named magnetic sources:
X (tangential to the geoid or the reference ellipsoid, towards the geographical North),
Y (tangential to the geoid or the reference ellipsoid, towards the geographical east) and,
Z (vertical, towards the centre of the Earth).
</skos:definition><skos:definition xml:lang="fr">Les coordonnées du vecteur champ magnétique en un point de l'espace en dehors des sources magnétiques nommées par convention :
X (tangentielle au géoide ou l'ellipsoide de référence, vers le Nord géographique),
Y (tangentielle au géoide ou l'ellipsoide de référence, vers l'Est géographique) et,
Z (verticale, vers le centre de la Terre).</skos:definition><skos:broader rdf:resource="geomagnetism-magnetic_field"/></skos:Concept><skos:Concept rdf:about="geomagnetism-paleomagnetism" xml:base="https://w3id.org/formater/variable/"><skos:prefLabel xml:lang="en">Paleomagnetism</skos:prefLabel><skos:prefLabel xml:lang="fr">Paléomagnétisme</skos:prefLabel><skos:definition xml:lang="en">Pertaining to the use of remnant magnetic signatures within the rocks of the Earth's crust to determine the state of the Earth's magnetic field at a given time into the past.</skos:definition><skos:definition xml:lang="fr">Utilisation de signatures magnétiques résiduelles dans les roches de la croûte terrestre pour déterminer l'état du champ magnétique terrestre à un moment donné dans le passé.
</skos:definition><skos:broader rdf:resource="geomagnetism"/><skos:exactMatch rdf:resource="https://gcmdservices.gsfc.nasa.gov/kms/concept/720969dd-e966-41aa-af94-ee41cdf60390"/></skos:Concept><skos:Concept rdf:about="geomagnetism-electrical_field" xml:base="https://w3id.org/formater/variable/"><skos:prefLabel xml:lang="en">Electrical field</skos:prefLabel><skos:prefLabel xml:lang="fr">Champ électrique </skos:prefLabel><skos:definition xml:lang="en">The electric force per unit charge. The direction of the field is taken to be the direction of the force it would exert on a positive test charge. The electric field is radially outward from a positive charge and radially in toward a negative point charge.</skos:definition><skos:definition xml:lang="fr"/><skos:broader rdf:resource="geomagnetism"/><skos:narrower rdf:resource="geomagnetism-electrical_field-electrical_intensity"/><skos:narrower rdf:resource="geomagnetism-electrical_field-electrical_anomalies"/><skos:exactMatch rdf:resource="https://gcmdservices.gsfc.nasa.gov/kms/concept/3202dab6-144a-4bfb-9bda-9d07e5ee7ec2"/></skos:Concept><skos:Concept rdf:about="geomagnetism-electrical_field-electrical_intensity" xml:base="https://w3id.org/formater/variable/"><skos:prefLabel xml:lang="en">Electrical intensity</skos:prefLabel><skos:prefLabel xml:lang="fr">Intensité électrique </skos:prefLabel><skos:definition xml:lang="en">The ratio of the electrostatic force exerted on a body to the charge on the body.</skos:definition><skos:definition xml:lang="fr"/><skos:broader rdf:resource="geomagnetism-electrical_field"/><skos:exactMatch rdf:resource="https://gcmdservices.gsfc.nasa.gov/kms/concept/84d77f98-d5a2-4da8-9ba6-0b15e082d050"/></skos:Concept><skos:Concept rdf:about="geomagnetism-electrical_field-electrical_anomalies" xml:base="https://w3id.org/formater/variable/"><skos:prefLabel xml:lang="en">Electrical anomalies</skos:prefLabel><skos:prefLabel xml:lang="fr">Anomalies électriques </skos:prefLabel><skos:definition xml:lang="en">A deviation from the normal or common order or form or rule.</skos:definition><skos:definition xml:lang="fr"/><skos:broader rdf:resource="geomagnetism-electrical_field"/><skos:exactMatch rdf:resource="https://gcmdservices.gsfc.nasa.gov/kms/concept/d55d29e8-9015-4c23-b137-528eb298aa49"/></skos:Concept><skos:Concept rdf:about="geomagnetism-geomagnetic_forecasts" xml:base="https://w3id.org/formater/variable/"><skos:prefLabel xml:lang="en">Geomagnetic forecasts</skos:prefLabel><skos:prefLabel xml:lang="fr">Geomagnetic forecasts</skos:prefLabel><skos:definition xml:lang="en">Forecasts of the likelihood (from 1% to 99%) that the daily geomagnetic activity level will reach a particular activity category. The four categories are Quiet to Unsettled, Active, Minor Storm, and Major to Severe Storm. The geomagnetic category assigned to a day is determined by the highest observed k-index for the day. Quiet to Unsettled = k 0 to k 3, Active = k 4, Minor Storm = k 5, and Major to Severe Storm = k 6 to k 9. Middle-latitude forecasts are verified against Fredericksburg, VA observations and High-latitude forecasts are verified against College, AK observations. Forecast lead times range from one to three days.</skos:definition><skos:definition xml:lang="fr"/><skos:broader rdf:resource="geomagnetism"/><skos:narrower rdf:resource="geomagnetism-geomagnetic_forecasts-total_intensity"/><skos:narrower rdf:resource="geomagnetism-geomagnetic_forecasts-geomagnetic_activity"/><skos:narrower rdf:resource="geomagnetism-geomagnetic_forecasts-geomagnetic_storm_category"/><skos:exactMatch rdf:resource="https://gcmdservices.gsfc.nasa.gov/kms/concept/02290e22-24ae-40f6-96f1-0c6c76a145af"/></skos:Concept><skos:Concept rdf:about="geomagnetism-geomagnetic_forecasts-total_intensity" xml:base="https://w3id.org/formater/variable/"><skos:prefLabel xml:lang="en">Total intensity</skos:prefLabel><skos:prefLabel xml:lang="fr">Total intensity</skos:prefLabel><skos:definition xml:lang="en">The magnetic intensity of the Earth's pull on an object, such as a satellite and measured by

X (easterly intensity),

Y (northerly intensity) and,

Z (vertical intensity, positive downwards).</skos:definition><skos:definition xml:lang="fr"/><skos:broader rdf:resource="geomagnetism-geomagnetic_forecasts"/><skos:exactMatch rdf:resource="https://gcmdservices.gsfc.nasa.gov/kms/concept/9a46a62c-952d-4253-8249-7375c14068a2"/></skos:Concept><skos:Concept rdf:about="geomagnetism-geomagnetic_forecasts-geomagnetic_activity" xml:base="https://w3id.org/formater/variable/"><skos:prefLabel xml:lang="en">Geomagnetic activity</skos:prefLabel><skos:prefLabel xml:lang="fr">Geomagnetic activity</skos:prefLabel><skos:definition xml:lang="en">Natural variations in the geomagnetic field classified into quiet, unsettled, active, and geomagnetic storm levels.</skos:definition><skos:definition xml:lang="fr"/><skos:broader rdf:resource="geomagnetism-geomagnetic_forecasts"/><skos:exactMatch rdf:resource="https://gcmdservices.gsfc.nasa.gov/kms/concept/2d3d9a57-44e8-43c0-98b4-b4891c994862"/></skos:Concept><skos:Concept rdf:about="geomagnetism-geomagnetic_forecasts-geomagnetic_storm_category" xml:base="https://w3id.org/formater/variable/"><skos:prefLabel xml:lang="en">Geomagnetic storm category</skos:prefLabel><skos:prefLabel xml:lang="fr">Geomagnetic storm category</skos:prefLabel><skos:definition xml:lang="en">A category or scale that describe the environmental disturbances for three event types: geomagnetic storms, solar radiation storms, and radio blackouts. The scales have numbered levels, analogous to hurricanes, tornadoes, and earthquakes that convey severity. They list possible effects at each level. They also show how often such events happen, and give a measure of the intensity of the physical causes.</skos:definition><skos:definition xml:lang="fr"/><skos:broader rdf:resource="geomagnetism-geomagnetic_forecasts"/><skos:exactMatch rdf:resource="https://gcmdservices.gsfc.nasa.gov/kms/concept/4b7decec-e378-4824-aecf-9fe509392efd"/></skos:Concept><skos:Concept rdf:about="solid_earth" xml:base="https://w3id.org/formater/variable/"><skos:prefLabel xml:lang="en">Solid Earth</skos:prefLabel><skos:prefLabel xml:lang="fr">Terre Solide</skos:prefLabel><skos:definition xml:lang="en">Refers to the Earth beneath our feet, the planet's solid surface and its interior.</skos:definition><skos:definition xml:lang="fr">La surface solide de la planète et son intérieur</skos:definition><skos:narrower rdf:resource="geomagnetism"/><skos:exactMatch rdf:resource="https://gcmdservices.gsfc.nasa.gov/kms/concept/2b9ad978-d986-4d63-b477-0f5efc8ace72"/></skos:Concept></rdf:RDF>